Seccompall.v
@@ -1,9 +1,32 @@
 Require Import Seccompfilter.
 Require Import Stackuse.
 Require Import compcert.driver.Compiler.
+Require Import compcert.common.Errors.
+Require Import compcert.common.AST.
+Require Import List.
+Require Import ZArith.
+
+Open Local Scope error_monad_scope.
 
 Definition bpf_to_asm (p: Seccomp.program) : res Asm.program :=
   do cmp <- Seccompfilter.transl_program_filter p;
   do asp <- Compiler.transf_cminor_program cmp;
   do asp' <- Stackuse.check_program asp;
-  asp'.
+  OK asp'.
+
+Theorem bpf_to_asm_stackok: forall p p', bpf_to_asm p = OK p' ->
+  forall id f, In (id, Gfun (Internal f)) (prog_defs p') ->
+  forall sz, stacksize f = OK sz -> (sz <= MaxStackSize)%Z.
+Proof.
+  intros.
+  eapply bounded_stack_useage; [|eauto].
+  monadInv H.
+  unfold check_program in *.
+  edestruct transform_partial_program_function; eauto.
+  destruct H.
+  destruct x1; simpl in *; try congruence.
+  monadInv H2.
+  rewrite EQ2.
+  monadInv EQ2.
+  destruct (Coqlib.zle x2 MaxStackSize); congruence.
+Qed.
